Extending arithmetic constraints to nested expressions, min & max.

checker/coq/arith.v
@@ -12,6 +12,7 @@ Require arith_ops.
 (* Propagation for multiplication.
  * We're not doing full factorization, just bounds. *)
 
+(*
 Inductive int_term :=
   | Const : Z -> int_term
   | Var : ivar -> int_term.
@@ -27,7 +28,102 @@ Definition domset_term_dbound term ds :=
   | Const c => (Bounded c, Bounded c)
   | Var x => (fst (var_dom ds x))
   end.
+*)
 
+Inductive binop := Plus | Times | Sub | Div | Min | Max.
+
+Definition rel_of f : Z -> Z -> Z -> Prop := fun z x y => Z.eq z (f x y).
+Definition part_of (f : Z -> Z -> Z) :=
+  fun x y => match x, y with
+               | Some x', Some y' => Some (f x' y')
+               | None, _ => None
+               | _, None => None
+             end.
+
+Definition binop_rel op :=
+   match op with
+     | Plus => rel_of Z.add
+     | Times => rel_of Z.mul
+     | Sub => rel_of Z.sub
+     | Div => fun z x y => y <> 0%Z /\ z = Z.quot x y
+     | Min => rel_of Z.min
+     | Max => rel_of Z.max
+   end.
+  
+Definition binop_pfun op :=
+  match op with
+    | Plus => part_of Z.add
+    | Times => part_of Z.mul
+    | Sub => part_of Z.sub
+    | Div =>
+      (fun x y =>
+         match x, y with
+           | Some x, Some y =>
+             if Z.eqb y 0%Z then
+               None
+             else
+               Some (Z.quot x y)
+           | None, _ => None
+           | _, None => None
+         end)
+    | Min => part_of Z.min
+    | Max => part_of Z.max
+  end.
+    
+Inductive aexpr :=
+| T : iterm -> aexpr
+| Op : binop -> aexpr -> aexpr -> aexpr.
+
+Fixpoint eval_aexpr exp theta v :=
+  match exp with
+    | T t => v = eval_iterm t theta
+    | Op op x y =>
+      exists x' y', eval_aexpr x theta x' /\ eval_aexpr y theta y' /\ binop_rel op v x' y'
+  end.
+
+Definition arith_eq := (iterm * aexpr)%type.
+Definition eval_arith_eq aeq theta := eval_aexpr (snd aeq) theta (eval_iterm (fst aeq) theta).
+
+Definition db_of_binop op : dbound -> dbound -> dbound :=
+   match op with
+     | Plus => db_add
+     | Times => arith_ops.db_mul
+     | Sub => fun x y => db_add x (arith_ops.db_neg y)
+     | Div => fun x y => arith_ops.db_div x y
+     | Min => db_min
+     | Max => db_max
+   end.
+Lemma db_of_binop_spec : forall op x x' k k' r, sat_dbound x k -> sat_dbound x' k' -> binop_rel op r k k' -> sat_dbound (db_of_binop op x x') r.
+Proof.
+  intros op x x' k k' r.
+  unfold binop_rel, db_of_binop, rel_of; destruct op; intros Hx Hx' Hr; try rewrite Hr.
+  + apply db_impl_adddb; intuition.
+  + apply arith_ops.db_mul_sound; assumption.
+  + apply arith_ops.db_neg_valid in Hx'.
+    apply db_impl_adddb; intuition.
+  + destruct Hr as [H0 Hr].
+    rewrite Hr; apply arith_ops.db_div_sound; assumption.
+  + apply range.db_min_spec; assumption.
+  + apply range.db_max_spec; assumption.
+Qed.
+
+Fixpoint db_of_aexpr exp ds :=
+  match exp with
+  | T t => range_of_dom (term_dom ds t)
+  | Op op x y => db_of_binop op (db_of_aexpr x ds) (db_of_aexpr y ds)
+  end.
+Lemma db_of_aexpr_spec : forall exp ds theta r, eval_domset ds theta -> eval_aexpr exp theta r -> sat_dbound (db_of_aexpr exp ds) r.
+Proof.
+  intros exp ds theta r Hds.
+  generalize r; clear r.
+  induction exp; intro r; unfold db_of_aexpr, eval_aexpr; fold db_of_aexpr; fold eval_aexpr.
+  + intro Hr; rewrite Hr.
+    apply term_dom_valid; assumption.
+  + intro Hxy; elim Hxy; clear Hxy; intros x' Hy; elim Hy; clear Hy; intros y' Hxy; destruct Hxy as [Hx [Hy Hr]].
+    apply db_of_binop_spec with (k := x') (k' := y'); try (apply IHexp1 || apply IHexp2); try assumption.
+Qed.    
+  
+(*
 Inductive int_arith :=
   | Mul : ivar -> ivar -> ivar -> int_arith
   | Div : ivar -> ivar -> ivar -> int_arith.
@@ -39,20 +135,82 @@ Definition eval_int_arith arith theta :=
   | Div x y z =>
     (eval_ivar z theta) <> 0 /\ (eval_ivar x theta) = Z.quot (eval_ivar y theta) (eval_ivar z theta)
   end.
+*)
 
-Definition ArithConstraint := mkConstraint int_arith eval_int_arith.
+Definition ArithConstraint := mkConstraint arith_eq eval_arith_eq.
 
 (* What are the semantics of Div?
    - Round towards zero/round towards -infty?
    - x/0 fails? or x/0 = 0?
    Most sense to have round-towards-zero, x/0 fails. *)
+(*
 Definition check_int_arith_sol arith theta :=
   match arith with
   | Mul x y z => Z.eqb (eval_ivar x theta) ((eval_ivar y theta)*(eval_ivar z theta))
   | Div x y z =>
     andb (negb (Z.eqb (eval_ivar z theta) 0)) (Z.eqb (eval_ivar x theta) (Z.quot (eval_ivar y theta) (eval_ivar z theta)))
   end.
+*)
 
+Fixpoint eval_aexpr_part expr theta :=
+  match expr with
+    | T t => Some (eval_iterm t theta)
+    | Op op x y =>
+      binop_pfun op (eval_aexpr_part x theta) (eval_aexpr_part y theta)
+  end.
+Lemma eval_aexpr_part_sound : forall expr theta r, eval_aexpr_part expr theta = Some r -> eval_aexpr expr theta r.
+Proof.
+  intros expr theta; induction expr; intro r.
+  + unfold eval_aexpr_part, eval_aexpr; intro Hr; inversion Hr; now rewrite H0.
+  + unfold eval_aexpr_part, eval_aexpr; fold eval_aexpr_part; fold eval_aexpr.
+    remember (eval_aexpr_part expr1 theta) as Ok; remember (eval_aexpr_part expr2 theta) as Ok'.
+    unfold binop_pfun, part_of, binop_rel, rel_of; destruct b, Ok, Ok'; intro Hr; try congruence; inversion Hr;
+    specialize (IHexpr1 v); specialize (IHexpr2 v0);
+    exists v, v0; try intuition.
+    rewrite H2 in Hr; simpl in Hr; congruence.
+    eqelim (Z.eqb v0 0); try congruence.
+Qed.
+    
+Definition check_arith_sol arith theta :=
+  match eval_aexpr_part (snd arith) theta with
+    | None => false
+    | Some r => Z.eqb r (eval_iterm (fst arith) theta)
+  end.
+Lemma check_arith_sol_valid : forall arith theta, check_arith_sol arith theta = true -> eval_arith_eq arith theta.
+Proof.
+  intros arith theta.
+  unfold check_arith_sol, eval_arith_eq.
+  eqelim (eval_aexpr_part (snd arith) theta).
+  intro Hb; apply eval_aexpr_part_sound.
+  rewrite Z.eqb_eq in Hb.
+  congruence.
+  intros; congruence.
+Qed.
+
+Definition check_int_arith arith ds :=
+  unsatb_db (db_meet (range_of_dom (term_dom ds (fst arith))) (db_of_aexpr (snd arith) ds)).
+Lemma check_int_arith_valid : forall arith ds, check_int_arith arith ds = true -> cst_is_unsat ArithConstraint arith ds.
+Proof.
+  intros arith ds; unfold check_int_arith, cst_is_unsat, eval; simpl; unfold eval_arith_eq; destruct arith; simpl.
+  intros Hu theta Hds He.
+  rewrite unsatb_db_true_iff in Hu.
+  unfold unsat_db in Hu.
+  assert (sat_dbound (db_meet (range_of_dom (term_dom ds i)) (db_of_aexpr a ds)) (eval_iterm i theta)).
+  apply db_sat_impl_meet; split.
+  apply term_dom_valid; assumption.
+  apply db_of_aexpr_spec with (theta := theta); try assumption.
+  specialize (Hu (eval_iterm i theta)); contradiction.
+Qed.
+
+Definition ArithCheck :=
+  mkUnsatChecker ArithConstraint (check_int_arith) (check_int_arith_valid).
+
+(*
+Definition ArithDbnd := DomboundedConstraint ArithConstraint.
+Definition ArithDbndCheck := DomboundedDBCheck ArithConstraint ArithDSet.
+*)
+
+(*
 Definition check_int_arith arith (ds : domset) :=
   match arith with
   | Mul x y z =>
@@ -62,7 +220,9 @@ Definition check_int_arith arith (ds : domset) :=
          (arith_ops.db_mul (db_from_dom y ds) (db_from_dom z ds)))
   | Div x y z => negb (arith_ops.db_div_check (db_from_dom x ds) (db_from_dom y ds) (db_from_dom z ds))
   end.
+*)
 
+(*
 Theorem check_int_arith_valid :
   forall (arith : int_arith) (ds : domset),
     check_int_arith arith ds = true -> cst_is_unsat ArithConstraint arith ds.
@@ -101,6 +261,7 @@ Proof.
 Qed.
 
 Definition ArithCheck := mkUnsatChecker ArithConstraint (check_int_arith) (check_int_arith_valid).
+*)
 
 (*
 Definition check_int_arith_dbfun arith (f : dbfun) :=
@@ -140,6 +301,7 @@ Definition check_reif_arith_dbnd (r : lit) (a : int_arith) (ds : domset) (cl : c
   (check (reif.ReifiedConstraint ArithDbnd) (reif.ReifiedCheck ArithDbnd ArithDomCheck)) (r, (ds, a)) cl.
 *)
 
+(*
 Theorem eval_int_arith_sol_valid :
     forall arith theta,
       (check_int_arith_sol arith theta = true) -> eval_int_arith arith theta.
@@ -150,5 +312,6 @@ Proof.
   intro H; destruct H as [H0 Hquot].
   split; [intro Heq ; rewrite <- Z.eqb_eq in Heq; now rewrite Heq in H0 | assumption].
 Qed.
+*)
 
-Definition ArithSolCheck := mkSolChecker ArithConstraint check_int_arith_sol eval_int_arith_sol_valid.
+Definition ArithSolCheck := mkSolChecker ArithConstraint check_arith_sol check_arith_sol_valid.
